Lean/Geo/Hexagon/Encoding.lean
@@ -23,14 +23,14 @@ def no6Hole4Above (a d e f : Fin n) : PropForm (Var n) :=
 def no6HoleClauses1 (n : Nat) (holes : Bool) : PropForm (Var n) :=
   .forAll (Fin n) fun a =>
   .forAll (Fin n) fun b =>
-  .guard (a.1+1 < b.1) fun _ =>
+  .impP (a.1+1 < b.1) fun _ =>
   .forAll (Fin n) fun c =>
-  .guard (b < c) fun _ =>
+  .impP (b < c) fun _ =>
   .forAll (Fin n) fun d =>
-  .guard (c < d) fun _ =>
+  .impP (c < d) fun _ =>
   .flatCNF <| .all #[
     no6Hole3Below holes a b c d,
-    .guard (a.1+2 < b.1) fun _ => no6Hole4Above a b c d
+    .impP (a.1+2 < b.1) fun _ => no6Hole4Above a b c d
   ]
 
 --     ·   c'
@@ -38,7 +38,7 @@ def no6HoleClauses1 (n : Nat) (holes : Bool) : PropForm (Var n) :=
 --     ·   c
 def no6Hole2Below (holes : Bool) (a c d c' : Fin n) : PropForm (Var n) :=
   .not <| .all #[Var.cup a c d, Var.cap a c' d,
-    .guard holes fun _ => if c < c' then Var.hole a c c' else Var.hole a c' c]
+    .impP holes fun _ => if c < c' then Var.hole a c c' else Var.hole a c' c]
 
 --        ·
 --   ·         d
@@ -50,14 +50,14 @@ def no6Hole1Below (a d e p : Fin n) : PropForm (Var n) :=
 def no6HoleClauses2 (n : Nat) (holes : Bool) : PropForm (Var n) :=
   .forAll (Fin n) fun a =>
   .forAll (Fin n) fun b =>
-  .guard (a.1 + 1 < b.1) fun _ =>
+  .impP (a.1 + 1 < b.1) fun _ =>
   .forAll (Fin n) fun c =>
-  .guard (b < c) fun _ =>
+  .impP (b < c) fun _ =>
   .forAll (Fin n) fun p =>
-  .guard (a < p ∧ p < c ∧ b ≠ p) fun _ =>
+  .impP (a < p ∧ p < c ∧ b ≠ p) fun _ =>
   .all #[
-    .guard (a.1 + 1 < p.1) fun _ => no6Hole2Below holes a b c p,
-    .guard (a.1 + 2 < b.1) fun _ => no6Hole1Below a b c p
+    .impP (a.1 + 1 < p.1) fun _ => no6Hole2Below holes a b c p,
+    .impP (a.1 + 2 < b.1) fun _ => no6Hole1Below a b c p
   ]
 
 def hexagonEncoding (n : Nat) (holes : Bool) : PropForm (Var n) :=
