Lean/Geo/KGon/Encoding.lean
@@ -11,11 +11,11 @@ def signotopeClauses1 (n : Nat) : PropForm (Var n) :=
   -- for all `a`, `b`, `c` with `a < b < c`
   .forAll (Fin n) fun a =>
   .forAll (Fin n) fun b =>
-  .guard (a < b) fun _ =>
+  .impP (a < b) fun _ =>
   .forAll (Fin n) fun c =>
-  .guard (b < c) fun _ =>
+  .impP (b < c) fun _ =>
   .forAll (Fin n) fun d =>
-  .guard (c < d) fun _ =>
+  .impP (c < d) fun _ =>
   .all #[
     -- (s{a, b, c} ∧ s{a, c, d}) → s{a, b, d} -- 1.1
     .imp (.and (sigma a b c) (sigma a c d)) (sigma a b d),
@@ -27,11 +27,11 @@ def signotopeClauses2 (n : Nat) : PropForm (Var n) :=
   -- for all `a`, `b`, `c` with `a < b < c`
   .forAll (Fin n) fun a =>
   .forAll (Fin n) fun b =>
-  .guard (a < b) fun _ =>
+  .impP (a < b) fun _ =>
   .forAll (Fin n) fun c =>
-  .guard (b < c) fun _ =>
+  .impP (b < c) fun _ =>
   .forAll (Fin n) fun d =>
-  .guard (c < d) fun _ =>
+  .impP (c < d) fun _ =>
   .all #[
     -- (s{a, b, c} ∧ s{b, c, d}) → s{a, c, d} -- 2.1
     .imp (.and (sigma a b c) (sigma b c d)) (sigma a c d),
@@ -43,19 +43,19 @@ def insideClauses (n : Nat) : PropForm (Var n) :=
   -- for all `a`, `b`, `c` with `a < b < c`
   .forAll (Fin n) fun a =>
   .forAll (Fin n) fun b =>
-  .guard (a < b) fun _ =>
+  .impP (a < b) fun _ =>
   .forAll (Fin n) fun c =>
-  .guard (b < c) fun _ =>
+  .impP (b < c) fun _ =>
   .forAll (Fin n) fun i =>
   .flatCNF <| .all #[
     -- a < x < b
-    .guard (a < i ∧ i < b) fun _ =>
+    .impP (a < i ∧ i < b) fun _ =>
       -- NOTE(Bernardo): Each of those should be expressible as 8 clauses or so
       -- I{i, a, b, c} ↔ ((s{a, b, c} ↔ s{a, i, c}) ∧ (!s{a, i, b} ↔ s{a, b, c}))
       .imp (inside i a b c) (
         .and (.iff (sigma a b c) (sigma a i c)) (.iff (sigma a b c) (.not (sigma a i b))))
   , -- b < i < c
-    .guard (b < i ∧ i < c) fun _ =>
+    .impP (b < i ∧ i < c) fun _ =>
       -- I{i, a, b, c} ↔ ((s{a, b, c} ↔ s{a, i, c}) ∧ (!s{b, i, c} ↔ s{a, b, c}))
       .imp (inside i a b c) (
         .and (.iff (sigma a b c) (sigma a i c)) (.iff (sigma a b c) (.not (sigma b i c))))
@@ -64,22 +64,22 @@ def insideClauses (n : Nat) : PropForm (Var n) :=
 def holeDefClauses0 (n : Nat) : PropForm (Var n) :=
   .forAll (Fin n) fun b =>
   .forAll (Fin n) fun c =>
-  .guard (b < c) fun _ =>
+  .impP (b < c) fun _ =>
   .flatCNF <| .imp
     (.forAll (Fin n) fun x =>
-      .guard (b < x ∧ x < c) fun _ =>
+      .impP (b < x ∧ x < c) fun _ =>
       Var.sigma b x c)
     (Var.hole₀ 0 b c)
 
 def holeDefClauses1 (n : Nat) : PropForm (Var n) :=
   .forAll (Fin n) fun a =>
   .forAll (Fin n) fun b =>
-  .guard (a < b) fun _ =>
+  .impP (a < b) fun _ =>
   .forAll (Fin n) fun c =>
-  .guard (b < c) fun _ =>
+  .impP (b < c) fun _ =>
   .flatCNF <| .imp
     (.forAll (Fin n) fun i =>
-      .guard (a < i ∧ i < c ∧ i ≠ b) fun _ =>
+      .impP (a < i ∧ i < c ∧ i ≠ b) fun _ =>
       .not (Var.inside i a b c))
     (Var.hole a b c)
 
@@ -94,16 +94,16 @@ def revLexClausesCore (F : Fin n → PropForm α) (a b : Fin n) (acc : PropForm 
     acc
 
 def revLexClauses (n : Nat) : PropForm (Var n) :=
-  .guard (4 ≤ n) fun _ =>
+  .impP (4 ≤ n) fun _ =>
   revLexClausesCore (n := n-2) ⟨0, by omega⟩ ⟨n - 3, by omega⟩ .true
     (F := fun ⟨a, _⟩ => Var.sigma ⟨a, by omega⟩ ⟨a+1, by omega⟩ ⟨a+2, by omega⟩)
 
 def baseEncoding (n : Nat) (holes : Bool) : PropForm (Var n) :=
   .all #[signotopeClauses1 n, revLexClauses n,
-    .guard holes fun _ => .and (insideClauses n) (holeDefClauses1 n)]
+    .impP holes fun _ => .and (insideClauses n) (holeDefClauses1 n)]
 
 def holeIf (holes : Bool) (a b c : Fin n) : PropForm (Var n) :=
-  .guard holes fun _ => Var.hole a b c
+  .impP holes fun _ => Var.hole a b c
 
 def arc' (o : Orientation) (sz : Nat) (a b c : Fin n) : PropForm (Var n) :=
   if sz = 0 then
@@ -126,19 +126,19 @@ def arc' (o : Orientation) (sz : Nat) (a b c : Fin n) : PropForm (Var n) :=
 def arcDefClauses1 (n : Nat) (o : Orientation) (sz : Nat) : PropForm (Var n) :=
   .forAll (Fin n) fun a =>
   .forAll (Fin n) fun b =>
-  .guard (a.1+sz < b.1) fun _ =>
+  .impP (a.1+sz < b.1) fun _ =>
   .forAll (Fin n) fun c =>
-  .guard (b < c) fun _ =>
+  .impP (b < c) fun _ =>
   .forAll (Fin n) fun d =>
-  .guard (c < d) fun _ =>
+  .impP (c < d) fun _ =>
   .imp (.and (arc' o sz a b c) (arc' o 0 b c d)) (Var.arc o (sz+1) a c d)
 
 def arcDefClauses2 (n : Nat) (o : Orientation) (sz : Nat) : PropForm (Var n) :=
   .forAll (Fin n) fun a =>
   .forAll (Fin n) fun c =>
-  .guard (a.1+sz < c.1) fun _ =>
+  .impP (a.1+sz < c.1) fun _ =>
   .forAll (Fin n) fun d =>
-  .guard (c < d) fun _ =>
+  .impP (c < d) fun _ =>
   .imp (Var.arc o (sz+1) a c d) (arc' o sz a c d)
 
 --                .   b
@@ -147,9 +147,9 @@ def arcDefClauses2 (n : Nat) (o : Orientation) (sz : Nat) : PropForm (Var n) :=
 def capFDefClauses (n : Nat) (holes : Bool) : PropForm (Var n) :=
   .forAll (Fin n) fun a =>
   .forAll (Fin n) fun b =>
-  .guard (a.1+1 < b.1) fun _ =>
+  .impP (a.1+1 < b.1) fun _ =>
   .forAll (Fin n) fun c =>
-  .guard (b < c) fun _ =>
+  .impP (b < c) fun _ =>
   .forAll (Fin n) fun d =>
-  .guard (c < d) fun _ =>
+  .impP (c < d) fun _ =>
   .imp (.all #[Var.cap a b c, .not (Var.sigma b c d), holeIf holes a b d]) (Var.capF a c d)
